Day 4: More Restructuring

Gaea/Peano/Nat.lean
@@ -1,17 +1,38 @@
+import Gaea.Syntax.Math
+
 universes u v
+
+open Gaea.Syntax
 
 namespace Gaea.Peano
 
-class Nat (prop : Sort u) (form : Sort v) := 
-  (nat : form -> prop)
+class IsNat (prop : Sort u) (form : Sort v) := 
+  (is_nat : form -> prop)
 
-export Nat (nat)
+namespace IsNat
+
+abbrev nat {P : Sort u} {T : Sort v} [C : IsNat P T] := C.is_nat
+
+def prop {P : Sort u} {T : Sort v} (N : IsNat P T) := P
+def form {P : Sort u} {T : Sort v} (N : IsNat P T) := T
+def pred {P : Sort u} {T : Sort v} (N : IsNat P T) := T -> P
+
+end IsNat
+
+export IsNat (nat)
+
+class Nat (P : Sort u) (T : Sort v) extends IsNat P T, Zero T, Succ T
 
 namespace Nat
 
 def prop {P : Sort u} {T : Sort v} (N : Nat P T) := P
 def form {P : Sort u} {T : Sort v} (N : Nat P T) := T
 def pred {P : Sort u} {T : Sort v} (N : Nat P T) := T -> P
+
+def nat {P : Sort u} {T : Sort v} (N : Nat P T) := N.toIsNat.is_nat
+def is_nat {P : Sort u} {T : Sort v} (N : Nat P T) := N.toIsNat.is_nat
+def zero {P : Sort u} {T : Sort v} (N : Nat P T) := N.toZero.zero
+def succ {P : Sort u} {T : Sort v} (N : Nat P T) := N.toSucc.S
 
 end Nat
 
