Gaea/Peano/Props.lean
@@ -18,58 +18,58 @@ namespace Gaea.Peano.Props
 --------------------------------------------------------------------------------
 
 -- Axiom 1
-def natZero {P : Sort u} (T : Type v) [Nat P T] [Zero T] : P :=
+def natZero {P : Sort u} (T : Type v) [IsNat P T] [Zero T] : P :=
   nat (0 : T)
 
 -- Axiom 2
 def eqNatRefl {P : Sort u} (T : Sort v) 
-  [Nat P T] [LEq P T] [LIf P] [LForall P T] : P :=
+  [IsNat P T] [LEq P T] [LIf P] [LForall P T] : P :=
   forall (x : T) => nat x -> x = x
 
 -- Axiom 3
 def eqNatSymm {P : Sort u} (T : Sort v) 
-  [Nat P T] [LEq P T] [LIf P] [LAnd P] [LForall P T] : P :=
+  [IsNat P T] [LEq P T] [LIf P] [LAnd P] [LForall P T] : P :=
   forall (x y : T) => nat x /\ nat y -> (x = y -> y = x)
 
 -- Axiom 4
 def eqNatTrans {P : Sort u} (T : Sort v) 
-  [Nat P T] [LEq P T] [LIf P] [LAnd P] [LForall P T] : P :=
+  [IsNat P T] [LEq P T] [LIf P] [LAnd P] [LForall P T] : P :=
   forall (x y z : T) => nat x /\ nat y /\ nat z -> (x = y /\ y = z -> x = z)
 
 -- Axiom 5
 def natEqNat {P : Sort u} (L : Logic P) (T : Sort v) 
-  [Nat P T] [LEq P T] [LIf P] [LAnd P] [LForall P T] : P :=
+  [IsNat P T] [LEq P T] [LIf P] [LAnd P] [LForall P T] : P :=
   forall (a b : T) => nat b /\ a = b -> nat a
 
 -- Axiom 6
 def natSuccNat {P : Sort u} (T : Sort v) 
-  [Nat P T] [Succ T] [LIf P] [LForall P T] : P :=
+  [IsNat P T] [Succ T] [LIf P] [LForall P T] : P :=
   forall (n : T) => nat n -> nat (S n)
 
 -- Axiom 7
 def eqNatIffEqSucc {P : Sort u} (T : Sort v) 
-  [LEq P T] [Succ T] [Nat P T] [LIf P] [LIff P] [LAnd P] [LForall P T] : P :=
+  [LEq P T] [Succ T] [IsNat P T] [LIf P] [LIff P] [LAnd P] [LForall P T] : P :=
   forall (m n : T) => nat m /\ nat n -> (m = n <-> S m = S n)
 
 -- Axiom 7a
 def eqNatToEqSucc {P : Sort u} (T : Sort v) 
-  [LEq P T] [Succ T] [Nat P T] [LIf P] [LAnd P] [LForall P T] : P :=
+  [LEq P T] [Succ T] [IsNat P T] [LIf P] [LAnd P] [LForall P T] : P :=
   forall (m n : T) => nat m /\ nat n -> (m = n -> S m = S n)
 
 -- Axiom 7b
 def eqSuccToEqNat {P : Sort u} (T : Sort v) 
-  [Nat P T] [LEq P T] [Succ T] [LIf P] [LAnd P] [LForall P T] : P :=
+  [IsNat P T] [LEq P T] [Succ T] [LIf P] [LAnd P] [LForall P T] : P :=
   forall (m n : T) => nat m /\ nat n -> (S m = S n -> m = n)
 
 -- Axiom 8
 def succNatEqZeroFalse {P : Sort u} (T : Type v) 
-  [Nat P T] [LEq P T] [False P] [Zero T] [Succ T] [LIf P] [LAnd P] [LForall P T] : P :=
+  [IsNat P T] [LEq P T] [False P] [Zero T] [Succ T] [LIf P] [LAnd P] [LForall P T] : P :=
   forall (m n : T) => nat m /\ nat n -> (S n = 0 -> false)
 
 -- Axiom 9
 def natInduction 
   {P : Sort u} (T : Type v) 
-  [Nat P T] [Zero T] [Succ T]
+  [IsNat P T] [Zero T] [Succ T]
   [LIf P] [LAnd P] [LForall P T] [LForall P (T -> P)]  : P := 
   forall (f : T -> P) => 
     f 0 -> 
@@ -82,12 +82,12 @@ def natInduction
 
 -- Axiom 1
 def addNatZeroEqNat {P : Sort u} (T : Type v) 
-  [Nat P T] [LEq P T] [Add T] [Zero T] [LIf P] [LForall P T] : P :=
+  [IsNat P T] [LEq P T] [Add T] [Zero T] [LIf P] [LForall P T] : P :=
   forall (a : T) => nat a -> a + 0 = a
 
 -- Axiom 2
 def addNatSuccEqSucc {P : Sort u} (T : Type v) 
-  [Nat P T] [LEq P T] [Add T] [Succ T] [LIf P] [LAnd P] [LForall P T] : P := 
+  [IsNat P T] [LEq P T] [Add T] [Succ T] [LIf P] [LAnd P] [LForall P T] : P := 
   forall (a b : T) => nat a /\ nat b -> a + S b = S (a + b)
 
 --------------------------------------------------------------------------------
@@ -96,12 +96,12 @@ def addNatSuccEqSucc {P : Sort u} (T : Type v)
 
 -- Axiom 1
 def mulNatZeroEqZero {P : Sort u} (T : Type v) 
-  [Nat P T] [LEq P T] [Mul T] [Zero T] [LIf P] [LForall P T] : P :=
+  [IsNat P T] [LEq P T] [Mul T] [Zero T] [LIf P] [LForall P T] : P :=
   forall (a : T) => nat a -> a * 0 = 0
 
 -- Axiom 2
 def mulNatSuccEqAddMul {P : Sort u} (T : Type v) 
-  [Nat P T] [LEq P T] [Add T] [Mul T] [Succ T] [LIf P] [LAnd P] [LForall P T] : P := 
+  [IsNat P T] [LEq P T] [Add T] [Mul T] [Succ T] [LIf P] [LAnd P] [LForall P T] : P := 
   forall (a b : T) => nat a /\ nat b -> a + S b = a + S (a * b)
 
 --------------------------------------------------------------------------------
@@ -111,14 +111,14 @@ def mulNatSuccEqAddMul {P : Sort u} (T : Type v)
 -- Axiom 1
 def leIffAddNat 
   {P : Sort u} (T : Type v) 
-  [Nat P T]  [LE P T] [LEq P T] [Add T] 
+  [IsNat P T]  [LE P T] [LEq P T] [Add T] 
   [LIf P] [LIff P] [LAnd P] [LForall P T] [LExists P T] : P :=
   forall (a b : T) => nat a /\ nat b -> (a <= b <-> exists c => nat c -> a + c = b)
 
 -- Axiom 2
 def strongNatInduction 
   {P : Sort u} (T : Type v) 
-  [Nat P T] [LE P T] [Zero T] [Succ T]
+  [IsNat P T] [LE P T] [Zero T] [Succ T]
   [LIf P] [LAnd P] [LForall P T] [LForall P (T -> P)] : P := 
   forall (f : T -> P) => 
     f 0 -> 
