Gaea/Peano/Rules.lean
@@ -11,104 +11,184 @@ universes u v w
 open Gaea.Logic
 open Gaea.Syntax
 
-namespace Gaea.Peano.Rules
+namespace Gaea.Peano
 
 --------------------------------------------------------------------------------
--- Natural Axioms
+-- Logic Rules
+--------------------------------------------------------------------------------
+
+def forallNatIntro {P : Sort u} {T : Type v} {L : Logic P} 
+  [N : IsNat P T] [Fa : LForall P T] [If : LIf P] [ForallIntro L Fa] [IfIntro L If]
+  {f : T -> P} (F : (a : T) -> (L |- nat a) -> (L |- f a))
+  : L |- forall a => nat a -> f a
+  := forallIntro fun a => ifIntro fun Na => F a Na
+
+def forallNatElim {P : Sort u} {T : Type v} {L : Logic P} 
+  [N : IsNat P T] [Fa : LForall P T] [If : LIf P] [ForallElim L Fa] [IfElim L If]
+  {f : T -> P} (p : L |- forall (a : T) => nat a -> f a) 
+  {a : T} (Na : L |- nat a) : L |- f a
+  := ifElim (forallElim p a) Na
+
+--------------------------------------------------------------------------------
+-- Natural Rules
 --------------------------------------------------------------------------------
 
 -- Axiom 1
-def NatZero  {P : Sort u} {T : Type v} 
-  (L : Logic P) (N : Nat P T) (Z : Zero T) :=
-  L |- nat (0 : T)
+class NatZero {P : Sort u} {T : Type v} 
+  (L : Logic P) (N : IsNat P T) (Z : Zero T) :=
+  (natZero : L |- nat (0 : T))
+
+namespace NatZero
+def nat0 {P : Sort u} {T : Type v} 
+  {L : Logic P} [N : IsNat P T] [Z : Zero T] [C : NatZero L N Z] := C.natZero
+end NatZero
+
+export NatZero (natZero nat0)
 
 -- Axiom 2
-def EqNatRefl {P : Sort u} {T : Sort v} 
-  (L : Logic P) (N : Nat P T) (Eq : LEq P T) :=
-  (x : T) -> (L |- nat x) -> (L |- x = x)
+class EqNatRefl {P : Sort u} {T : Sort v} 
+  (L : Logic P) (N : IsNat P T) (Eq : LEq P T) :=
+  (eqNatRefl : (x : T) -> (L |- nat x) -> (L |- x = x))
+
+export EqNatRefl (eqNatRefl)
 
 -- Axiom 3
-def EqNatSymm {P : Sort u} {T : Sort v} 
-  (L : Logic P) (N : Nat P T) (Eq : LEq P T) :=
-  (x y : T) -> (L |- nat x) -> (L |- nat y) ->
-    (L |- x = y) -> (L |- y = x)
+class EqNatSymm {P : Sort u} {T : Sort v} 
+  (L : Logic P) (N : IsNat P T) (Eq : LEq P T) :=
+  (eqNatSymm : (x y : T) -> (L |- nat x) -> (L |- nat y) ->
+    (L |- x = y) -> (L |- y = x))
+
+export EqNatSymm (eqNatSymm)
 
 -- Axiom 4
-def EqNatTrans {P : Sort u} {T : Sort v} 
-  (L : Logic P) (N : Nat P T) (Eq : LEq P T) :=
-  (x y z : T) -> (L |- nat x) -> (L |- nat y) -> (L |- nat z) -> 
-    (L |- x = y) -> (L |- y = z) -> (L |- x = z)
+class EqNatTrans {P : Sort u} {T : Sort v} 
+  (L : Logic P) (N : IsNat P T) (Eq : LEq P T) :=
+  (eqNatTrans : (x y z : T) -> (L |- nat x) -> (L |- nat y) -> (L |- nat z) -> 
+    (L |- x = y) -> (L |- y = z) -> (L |- x = z))
+
+export EqNatTrans (eqNatTrans)
 
 -- Axiom 5
-def NatEqNat {P : Sort u} {T : Sort v} 
-  (L : Logic P) (N : Nat P T) (Eq : LEq P T) :=
-  (a b : T) -> (L |- nat b) -> (L |- a = b) -> (L |- nat a)
+class NatEqNat {P : Sort u} {T : Sort v} 
+  (L : Logic P) (N : IsNat P T) (Eq : LEq P T) :=
+  (natEqNat : (a b : T) -> (L |- nat b) -> (L |- a = b) -> (L |- nat a))
+
+namespace NatEqNat
+def natEq {P : Sort u} {T : Sort v} 
+{L : Logic P} [N : IsNat P T] [Eq : LEq P T] [C : NatEqNat L N Eq] 
+{a b : T} : (L |- nat b) -> (L |- a = b) -> (L |- nat a) := C.natEqNat a b
+end NatEqNat
+
+export NatEqNat (natEqNat natEq)
 
 -- Axiom 6
-def NatSuccNat {P : Sort u} {T : Sort v} 
-  (L : Logic P) (N : Nat P T) (Su : Succ T) :=
-  (n : T) -> (L |- nat n) -> (L |- nat (S n))
+class NatSuccNat {P : Sort u} {T : Sort v} 
+  (L : Logic P) (N : IsNat P T) (Su : Succ T) :=
+  (natSuccNat : (n : T) -> (L |- nat n) -> (L |- nat (S n)))
+
+namespace NatSuccNat
+def natS {P : Sort u} {T : Sort v} 
+{L : Logic P} [N : IsNat P T] [Su : Succ T] [C : NatSuccNat L N Su] 
+{n : T} : (L |- nat n) -> (L |- nat (S n)) := C.natSuccNat n
+end NatSuccNat
+
+export NatSuccNat (natSuccNat natS)
 
 -- Axiom 7a
-def EqNatToEqSucc {P : Sort u} {T : Sort v} 
-  (L : Logic P) (N : Nat P T) (Eq : LEq P T) (Su : Succ T) :=
-  (m n : T) -> (L |- nat m) -> (L |- nat n) -> 
-    (L |- m = n) -> (L |- S m = S n)
+class EqNatToEqSucc {P : Sort u} {T : Sort v} 
+  (L : Logic P) (N : IsNat P T) (Eq : LEq P T) (Su : Succ T) :=
+  (eqNatToEqSucc : (m n : T) -> (L |- nat m) -> (L |- nat n) -> 
+    (L |- m = n) -> (L |- S m = S n))
+
+export EqNatToEqSucc (eqNatToEqSucc)
 
 -- Axiom 7b
-def EqSuccToEqNat {P : Sort u} {T : Sort v} 
-  (L : Logic P) (N : Nat P T) (Eq : LEq P T) (Su : Succ T) :=
-  (m n : T) -> (L |- nat m) -> (L |- nat n) -> 
-    (L |- S m = S n) -> (L |- m = n)
+class EqSuccToEqNat {P : Sort u} {T : Sort v} 
+  (L : Logic P) (N : IsNat P T) (Eq : LEq P T) (Su : Succ T) :=
+  (eqSuccToEqNat : (m n : T) -> (L |- nat m) -> (L |- nat n) -> 
+    (L |- S m = S n) -> (L |- m = n))
+
+export EqSuccToEqNat (eqSuccToEqNat)
 
 -- Axiom 8
-def SuccNatEqZeroFalse {P : Sort u} {T : Type v} 
-  (L : Logic P) (N : Nat P T) (Eq : LEq P T) (Z : Zero T) (Su : Succ T) [False P] :=
-  (m n : T) -> (L |- nat m) -> (L |- nat n) -> 
-    (L |- S n = 0) -> (L |- false)
+class SuccNatEqZeroFalse {P : Sort u} {T : Type v} 
+  (L : Logic P) (N : IsNat P T) (Eq : LEq P T) (Z : Zero T) (Su : Succ T) [False P] :=
+  (succNatEqZeroFalse : (m n : T) -> (L |- nat m) -> (L |- nat n) -> 
+    (L |- S n = 0) -> (L |- false))
+
+export SuccNatEqZeroFalse (succNatEqZeroFalse)
 
 -- Axiom 9
 -- Induction over predicates
-def NatInduction {P : Sort u} {T : Type v} 
-  (L : Logic P) (N : Nat P T) (Z : Zero T) (Su : Succ T) := 
-  (f : T -> P) -> (L |- f 0) -> 
-  ((n : T) -> (L |- nat n) -> (L |- f n) -> (L |- f (S n))) ->
-  ((n : T) -> (L |- nat n) -> (L |- f n))
+class NatInduction {P : Sort u} {T : Type v} 
+  (L : Logic P) (N : Nat P T) := 
+  (natInduction : 
+    (f : T -> P) -> (L |- f 0) -> 
+    ((n : T) -> (L |- nat n) -> (L |- f n) -> (L |- f (S n))) ->
+    ((n : T) -> (L |- nat n) -> (L |- f n)))
+
+def natInduction {P : Sort u} {T : Type v} 
+  {L : Logic P} [N : Nat P T] [I : NatInduction L N] := I.natInduction
 
 -- Axiom 9 (Alt)
 -- Induction over schemas
-def NatInduction' {P : Sort u} {T : Type v} 
-  (L : Logic P) (N : Nat P T) (Z : Zero T) (Su : Succ T) := 
-  (f : T -> Sort w) -> f 0 ->
-  ((n : T) -> (L |- nat n) -> (f n -> f (S n))) ->
-  ((n : T) -> (L |- nat n) -> f n)
+class NatInduction' {P : Sort u} {T : Type v} 
+  (L : Logic P) (N : Nat P T) := 
+  (natInduction' : (f : T -> Sort w) -> f 0 ->
+    ((n : T) -> (L |- nat n) -> (f n -> f (S n))) ->
+    ((n : T) -> (L |- nat n) -> f n))
+
+def natInduction' {P : Sort u} {T : Type v} 
+  (L : Logic P) [N : Nat P T] [I : NatInduction' L N] := I.natInduction'
 
 --------------------------------------------------------------------------------
--- Addition Axioms
---------------------------------------------------------------------------------
-
--- Axiom 1
-def AddNatZeroEqNat {P : Sort u} {T : Type v} 
-  (L : Logic P) (N : Nat P T) (Eq : LEq P T) (A : Add T) (Z : Zero T) :=
-  (a : T) -> (L |- nat a) -> (L |- a + 0 = a)
-
--- Axiom 2
-def AddNatSuccEqSucc {P : Sort u} {T : Type v} 
-  (L : Logic P) (N : Nat P T)  (Eq : LEq P T) (A : Add T) (Su : Succ T) := 
-  (a b : T) -> (L |- nat a) -> (L |- nat b) -> (L |- a + S b = S (a + b))
-
---------------------------------------------------------------------------------
--- Multiplication Axioms
+-- Addition Rules
 --------------------------------------------------------------------------------
 
 -- Axiom 1
-def MulNatZeroEqZero {P : Sort u} {T : Type v} 
-  (L : Logic P) (N : Nat P T) (Eq : LEq P T) (M : Mul T) (Z : Zero T)  :=
-  (a : T) -> (L |- nat a) -> (L |- a * 0 = 0)
+class AddNatZeroEqNat {P : Sort u} {T : Type v} 
+  (L : Logic P) (N : IsNat P T) (Eq : LEq P T) (A : Add T) (Z : Zero T) :=
+  (addNatZeroEqNat : (a : T) -> (L |- nat a) -> (L |- a + 0 = a))
+
+namespace AddNatZeroEqNat
+def An0_eq_n {P : Sort u} {T : Type v} 
+  {L : Logic P} [N : IsNat P T] [Eq : LEq P T] [A : Add T] [Z : Zero T] 
+  [C : AddNatZeroEqNat L N Eq A Z] {a : T} := C.addNatZeroEqNat a
+end AddNatZeroEqNat
+
+export AddNatZeroEqNat (addNatZeroEqNat An0_eq_n)
 
 -- Axiom 2
-def MulNatSuccEqAddMul {P : Sort u} {T : Type v} 
-  (L : Logic P) (N : Nat P T) (Eq : LEq P T) (M : Mul T) (A : Add T) (Su : Succ T) := 
-  (a b : T) -> (L |- nat a) -> (L |- nat b) -> (L |- a + S b = a + S (a * b))
+class AddNatSuccEqSucc {P : Sort u} {T : Type v} 
+  (L : Logic P) (N : IsNat P T) (Eq : LEq P T) (A : Add T) (Su : Succ T) := 
+  (addNatSuccEqSucc : (a b : T) -> (L |- nat a) -> (L |- nat b) -> 
+    (L |- a + S b = S (a + b)))
 
-end Gaea.Peano.Rules
+namespace AddNatSuccEqSucc
+def AmSn_eq_SAmn {P : Sort u} {T : Type v} 
+  {L : Logic P} [N : IsNat P T] [Eq : LEq P T] [A : Add T] [Su : Succ T]
+  [C : AddNatSuccEqSucc L N Eq A Su] {a b : T} := C.addNatSuccEqSucc a b
+end AddNatSuccEqSucc
+
+export AddNatSuccEqSucc (addNatSuccEqSucc AmSn_eq_SAmn)
+
+--------------------------------------------------------------------------------
+-- Multiplication Rules
+--------------------------------------------------------------------------------
+
+-- Axiom 1
+class MulNatZeroEqZero {P : Sort u} {T : Type v} 
+  (L : Logic P) (N : IsNat P T) (Eq : LEq P T) (M : Mul T) (Z : Zero T)  :=
+  (mulNatZeroEqZero : (a : T) -> (L |- nat a) -> (L |- a * 0 = 0))
+
+export MulNatZeroEqZero (mulNatZeroEqZero)
+
+-- Axiom 2
+class MulNatSuccEqAddMul {P : Sort u} {T : Type v} 
+  (L : Logic P) (N : IsNat P T) (Eq : LEq P T) (M : Mul T) (A : Add T) (Su : Succ T) := 
+  (mulNatSuccEqAddMul : (a b : T) -> (L |- nat a) -> (L |- nat b) -> 
+    (L |- a + S b = a + S (a * b)))
+
+export MulNatSuccEqAddMul (mulNatSuccEqAddMul)
+
+end Gaea.Peano
