Gaea/Peano/Theorems.lean
@@ -1,15 +1,12 @@
 import Gaea.Logic
 import Gaea.Syntax
-import Gaea.Syntax.Notation
-import Gaea.Logic.Rules
 import Gaea.Peano.Rules
+import Gaea.Peano.Modules
 
 universes u v w
 
 open Gaea.Logic
 open Gaea.Syntax
-open Gaea.Logic.Rules
-open Gaea.Peano.Rules
 
 namespace Gaea.Peano
 
@@ -17,18 +14,16 @@ namespace Gaea.Peano
 -- General Theorems
 --------------------------------------------------------------------------------
 
-def natCases 
-{P : Sort u} {T : Type v} {L : Logic P} 
-[Z : Zero T] [Su : Succ T] [N : Nat P T] 
-(natInduction : NatInduction L N Z Su)
+theorem natCases 
+{P : Sort u} {T : Type v} {L : Logic P} [N : Nat P T] [NatInduction L N]
 : (f : T -> P) -> 
   (L |- f 0) -> ((n : T) -> (L |- nat n) -> (L |- f (S n))) -> 
     ((n : T) -> (L |- nat n) -> (L |- f n))
 := by
-  intro f f0 fS n nat_n
+  intro f f0 fS n Nn
   have ih : (n : T) -> (L |- nat n) -> (L |- f n) -> (L |- f (S n)) := 
-    fun n nat_n fn => fS n nat_n
-  exact natInduction f f0 ih n nat_n
+    fun n Nn fn => fS n Nn
+  exact natInduction f f0 ih n Nn
 
 --------------------------------------------------------------------------------
 -- Addition Theorems
@@ -36,99 +31,62 @@ def natCases
 
 theorem addZeroEqZero 
 {P : Sort u} {T : Type v} {L : Logic P}
-[Eq : LEq P T] [A : Add T] [Z : Zero T] [N : Nat P T]
-(nat_0 : NatZero L N Z) 
-(An0_eq_n : AddNatZeroEqNat L N Eq A Z)
+[Q : LEq P T] [A : Add T] [Z : Zero T] [N : IsNat P T]
+[NatZero L N Z] [AddNatZeroEqNat L N Q A Z]
 : L |- 0 + 0 = (0 : T) 
-:= An0_eq_n 0 nat_0
+:= An0_eq_n nat0
 
 theorem natAddNatZero
 {P : Sort u} {T : Type v} {L : Logic P}
-[Eq : LEq P T] [A : Add T] [Z : Zero T] [N : Nat P T] 
-(natEq : NatEqNat L N Eq) 
-(An0_eq_n : AddNatZeroEqNat L N Eq A Z)
+[Q : LEq P T] [A : Add T] [Z : Zero T] [N : IsNat P T] 
+[NatEqNat L N Q] [AddNatZeroEqNat L N Q A Z]
 : (a : T) -> (L |- nat a) -> (L |- nat (a + 0))
-:= by
-  intro a nat_a
-  apply natEq _ a nat_a
-  exact An0_eq_n a nat_a
+:= by intro a Na; apply natEq Na; exact An0_eq_n Na
 
 -- Uses standard (predicate) induction
-theorem natAddNat_induct
-{P : Sort u} {T : Type v} {L : Logic P}
-[N : Nat P T] [Eq : LEq P T] [A : Add T] [Z : Zero T] [Su : Succ T] 
-[Fa : LForall P T] [If : LIf P] 
-(ifIntro : IfIntro L If)
-(ifElim : IfElim L If)
-(forallIntro : ForallIntro L Fa)
-(forallElim : ForallElim L Fa)
-(natEq : NatEqNat L N Eq) 
-(nat_S : NatSuccNat L N Su) 
-(natInduction : NatInduction L N Z Su)
-(An0_eq_n : AddNatZeroEqNat L N Eq A Z)
-(AnS_eq_S : AddNatSuccEqSucc L N Eq A Su)
+theorem natAddNat_induct {P : Sort u} {T : Type v} {L : Logic P}
+[N : Nat P T] [Q : LEq P T] [A : PAdd L N Q] [Fa : MForall L T] [If : MIf L]
+[NatEqNat L N.toIsNat Q] [NatSuccNat L N.toIsNat N.toSucc] [NatInduction L N]
 : (b : T) -> (L |- nat b) -> (L |- forall (a : T) => nat a -> nat (a + b))
 := by
-  intro b nat_b
+  intro n Nn
   apply natInduction 
     (fun b => forall (a : T) => nat a -> nat (a + b))
-  -- Base
-  apply forallIntro; intro a
-  apply ifIntro; intro nat_a
-  exact natAddNatZero natEq An0_eq_n a nat_a
+  exact forallNatIntro natAddNatZero
   -- Induction
-  intro a nat_a p_Nn_to_NAna
-  apply forallIntro; intro b
-  apply ifIntro; intro nat_b
-  have nat_Aba := ifElim _ _ (forallElim _ p_Nn_to_NAna b) nat_b 
-  have AbSa_eq_SAba := AnS_eq_S _ _ nat_b nat_a
-  have nat_SAba := nat_S _ nat_Aba
-  exact natEq _ _ nat_SAba AbSa_eq_SAba
-  exact nat_b
+  intro a Na p_Nn_to_NAna
+  apply forallNatIntro; intro b Nb
+  have AbSa_eq_SAba := AmSn_eq_SAmn Nb Na
+  have NAba := forallNatElim p_Nn_to_NAna Nb 
+  exact natEq (natS NAba) AbSa_eq_SAba
+  exact Nn
 
-theorem natAddNat
-{P : Sort u} {T : Type v} {L : Logic P} 
-[N : Nat P T] [Eq : LEq P T] [A : Add T] [Z : Zero T] [Su : Succ T]
-[Fa : LForall P T] [If : LIf P] 
-(ifIntro : IfIntro L If)
-(ifElim : IfElim L If)
-(forallIntro : ForallIntro L Fa)
-(forallElim : ForallElim L Fa)
-(natEq : NatEqNat L N Eq) 
-(nat_S : NatSuccNat L N Su) 
-(natInduction : NatInduction L N Z Su)
-(An0_eq_n : AddNatZeroEqNat L N Eq A Z)
-(AnS_eq_S : AddNatSuccEqSucc L N Eq A Su)
+theorem natAddNat {P : Sort u} {T : Type v} {L : Logic P} 
+[N : Nat P T] [Q : LEq P T] [A : PAdd L N Q] [Fa : MForall L T] [If : MIf L]
+[NatEqNat L N.toIsNat Q] [NatSuccNat L N.toIsNat N.toSucc] [NatInduction L N]
 : (a b : T) -> (L |- nat a) -> (L |- nat b) -> (L |- nat (a + b))
-:= by
-  intro a b nat_a nat_b
-  have h :=  natAddNat_induct ifIntro ifElim forallIntro forallElim  
-    natEq nat_S natInduction An0_eq_n AnS_eq_S b nat_b
-  exact ifElim _ _ (forallElim _ h a) nat_a
+:= fun a b Na Nb => forallNatElim (natAddNat_induct b Nb) Na
 
 -- Uses schema induction
 theorem natAddNat'
 {P : Sort u} {T : Type v} {L : Logic.{u,w} P}
-[N : Nat P T] [Eq : LEq P T]  [A : Add T] [Z : Zero T] [Su : Succ T] 
-(natEq : NatEqNat L N Eq) 
-(nat_S : NatSuccNat L N Su) 
-(natInduction : NatInduction'.{u,v,(imax (v+1) w)} L N Z Su)
-(An0_eq_n : AddNatZeroEqNat L N Eq A Z)
-(AnS_eq_S : AddNatSuccEqSucc L N Eq A Su)
+[N : Nat P T] [Q : LEq P T]  [A : PAdd L N Q]
+[NatEqNat L N.toIsNat Q] [NatSuccNat L N.toIsNat N.toSucc] 
+[NatInduction'.{u,v,(imax (v+1) w)} L N]
 : (a b : T) -> (L |- nat a) -> (L |- nat b) -> (L |- nat (a + b))
 := by
-  intro m n nat_m nat_n
-  apply natInduction
-    (fun b => (a : T) -> (L |- nat a) -> (L |- nat (a + b)))
+  intro m n Nm Nn
+  apply natInduction' L
+    (fun (b : T) => (a : T) -> (L |- nat a) -> (L |- nat (a + b)))
   -- Base
-  intro a nat_a
-  exact natAddNatZero natEq An0_eq_n a nat_a
+  intro a Na
+  exact natAddNatZero a Na
   -- Induction
-  intro a nat_a ih b nat_b
-  have nat_Aba := ih b nat_b 
-  have abSa_eq_Saba := AnS_eq_S _ _ nat_b nat_a
-  have nat_SAba := nat_S _ nat_Aba
-  exact natEq _ _ nat_SAba abSa_eq_Saba
-  exact nat_n; exact nat_m
+  intro a Na ih b Nb
+  have NAba := ih b Nb 
+  have AbSa_eq_SAba := AmSn_eq_SAmn Nb Na
+  have NSAba := natS NAba
+  exact natEq NSAba AbSa_eq_SAba
+  exact Nn; exact Nm
 
 end Gaea.Peano
