Gaea/Syntax/Math.lean
@@ -2,11 +2,21 @@ namespace Gaea.Syntax
 
 -- Numerics
 
-abbrev Zero (N : Type u) 
-  := OfNat N (natLit! 0)
+-- abbrev Zero (N : Type u) 
+--   := OfNat N (natLit! 0)
+
+class Zero (N : Sort u) :=
+  (zero : N)
+
+instance (N : Type u) [C : Zero N] : OfNat N (natLit! 0)
+  := {ofNat := C.zero}
 
 class Succ (N : Sort u) :=
-  (S : N -> N)
+  (succ : N -> N)
+
+namespace Succ
+abbrev S {N : Sort u} [C : Succ N] := C.succ
+end Succ
 
 -- Inequalities
 
