Gaea/Logic.lean
@@ -1,1 +1,3 @@
 import Gaea.Logic.Basic
+import Gaea.Logic.Rules
+import Gaea.Logic.Modules
