Gaea/Logic/Modules.lean
@@ -1,0 +1,51 @@
+import Gaea.Logic.Basic
+import Gaea.Logic.Rules
+import Gaea.Syntax.Logic
+import Gaea.Logic.Notation
+import Gaea.Syntax.Notation
+
+universes u v
+
+open Gaea.Syntax
+
+namespace Gaea.Logic
+
+-- Forall
+
+class MForall {P : Sort u} (L : Logic P) (T : Sort v) extends LForall P T :=
+  (toForallIntro : ForallIntro L toLForall)
+  (toForallElim : ForallElim L toLForall)
+
+instance {P : Sort u} {T : Sort v} {L : Logic P} {C : MForall L T} :
+  ForallIntro L C.toLForall := {forallIntro := C.toForallIntro.forallIntro}
+
+instance {P : Sort u} {T : Sort v} {L : Logic P} {C : MForall L T} :
+  ForallElim L C.toLForall := {forallElim := C.toForallElim.forallElim}
+
+namespace MForall
+def forallIntro {P : Sort u} {T : Sort v} {L : Logic P} (C : MForall L T) 
+  := C.toForallIntro.forallIntro
+def ForallElim {P : Sort u} {T : Sort v} {L : Logic P} (C : MForall L T) 
+  := C.toForallElim.forallElim
+end MForall
+
+-- If
+
+class MIf {P : Sort u} (L : Logic P) extends LIf P :=
+  (toIfIntro : IfIntro L toLIf)
+  (toIfElim : IfElim L toLIf)
+
+instance {P : Sort u} {L : Logic P} {C : MIf L} :
+  IfIntro L C.toLIf := {ifIntro := C.toIfIntro.ifIntro}
+
+instance {P : Sort u} {L : Logic P} {C : MIf L} :
+  IfElim L C.toLIf := {ifElim := C.toIfElim.ifElim}
+
+namespace MIf
+def ifIntro {P : Sort u} {L : Logic P} {C : MIf L} 
+  := C.toIfIntro.ifIntro
+def ifElim {P : Sort u} {L : Logic P} {C : MIf L} 
+  := C.toIfElim.ifElim
+end MIf
+
+end Gaea.Logic
